Replica ID in interface

new/App_user_rc_do_merge_pre.fsti
@@ -1,4 +1,4 @@
-module App_user_rc
+module App_user_rc_do_merge_pre
 
 open FStar.Seq
 open FStar.Ghost
@@ -38,16 +38,15 @@ type log = seq op_t
 
 let get_rid (_,(rid,_)) = rid
 
+let mem_rid (rid:nat) (l:log) =
+  exists e. mem e l /\ fst (snd e) = rid
+  
 unfold
 let ( ++ ) (l1 l2:log) = Seq.append l1 l2
 
 unfold
 let mem_id (id:timestamp_t) (l:log) : bool =
   mem_assoc_fst id l
-
-unfold
-let mem_rid (rid:nat) (l:log) : bool =
-  mem_assoc_snd rid l
   
 unfold
 let distinct_ops (l:log) = distinct_assoc_fst l
@@ -57,23 +56,32 @@ type st0 = concrete_st & erased log
 let v_of (s:st0) : concrete_st = fst s
 let ops_of (s:st0) : GTot log = snd s
 
+//pre-condition for do
+val do_pre (s:concrete_st) (o:op_t) : prop
+
 // apply an operation to a state
-val do (s:concrete_st) (o:op_t) : concrete_st
+val do (s:concrete_st) (o:op_t{do_pre s o}) : concrete_st
 
 val lem_do (a b:concrete_st) (op:op_t)
-   : Lemma (requires eq a b)
-           (ensures eq (do a op) (do b op))
+   : Lemma (requires eq a b /\ do_pre a op)
+           (ensures do_pre b op /\ eq (do a op) (do b op))
 
+let rec do_pre_prop (x:concrete_st) (l:log) : Tot prop (decreases length l) =
+  match length l with
+  |0 -> True
+  |_ -> do_pre x (head l) /\ do_pre_prop (do x (head l)) (tail l)
+  
 // applying a log of operations to a concrete state
-let rec apply_log (x:concrete_st) (l:log) : Tot concrete_st (decreases length l) =
+let rec apply_log (x:concrete_st) (l:log{do_pre_prop x l}) : Tot concrete_st (decreases length l) =
   match length l with
   |0 -> x
   |_ -> apply_log (do x (head l)) (tail l)                   
 
 // property of apply_log
 let rec lem_apply_log (x:concrete_st) (l:log)
-  : Lemma (requires true)
-          (ensures (length l > 0 ==> (apply_log x l == apply_log (do x (head l)) (tail l)) /\
+  : Lemma (requires do_pre_prop x l)
+          (ensures (length l > 0 ==> do_pre_prop x (fst (un_snoc l)) /\ do_pre (apply_log x (fst (un_snoc l))) (last l) /\ 
+                                    (apply_log x l == apply_log (do x (head l)) (tail l)) /\
                                     (apply_log x l == do (apply_log x (fst (un_snoc l))) (last l))) /\
                    (length l = 0 ==> apply_log x l == x))
           (decreases length l) =
@@ -81,11 +89,12 @@ let rec lem_apply_log (x:concrete_st) (l:log)
   |0 -> ()
   |_ -> lem_apply_log (do x (head l)) (tail l)
 
-type st1 = s:st0{(v_of s == apply_log init_st (ops_of s))}
+type st1 = s:st0{do_pre_prop init_st (ops_of s) /\ (v_of s == apply_log init_st (ops_of s))}
 
 // valid state
 let valid_st (s:st0) : prop =
   distinct_ops (ops_of s) /\
+  do_pre_prop init_st (ops_of s) /\
   (v_of s == apply_log init_st (ops_of s))
 
 type st = s:st0{valid_st s}
@@ -96,7 +105,8 @@ val comm_ops (x y:op_t) : bool
 // if x and y are commutative ops, applying them in any order should give equivalent results
 val commutative_prop (x y:op_t) 
   : Lemma (requires comm_ops x y)
-          (ensures (forall s. eq (apply_log s (cons x (cons y empty))) (apply_log s (cons y (cons x empty)))))
+          (ensures (forall s. do_pre_prop s (cons x (cons y empty)) /\ do_pre_prop s (cons y (cons x empty)) ==>
+                         eq (apply_log s (cons x (cons y empty))) (apply_log s (cons y (cons x empty)))))
 
 //commutativity for a sequence of operation
 let commutative_seq (x:op_t) (l:log) : bool =
@@ -109,8 +119,11 @@ type rc_res =
 //conflict resolution
 val rc (x:op_t) (y:op_t{fst x <> fst y /\ ~ (comm_ops x y)}) : rc_res
 
+//pre-condition for merge
+val merge_pre (l a b:concrete_st) : prop
+
 // concrete merge operation
-val merge (l a b:concrete_st) : concrete_st
+val merge (l a:concrete_st) (b:concrete_st{merge_pre l a b}) : concrete_st
 
 // returns true if there exists an operation op in log l such that
 // 1. last_op and op are non-commutative
@@ -129,8 +142,9 @@ let reorder (last_op:op_t) (l:log)
                               commutative_seq op suf)) l
 
 let rec split_prefix (s:concrete_st) (l:log) (a:log)
-  : Lemma (requires is_prefix l a)
-          (ensures (apply_log s a == apply_log (apply_log s l) (diff a l)) /\
+  : Lemma (requires is_prefix l a /\ do_pre_prop s a)
+          (ensures do_pre_prop s l /\ do_pre_prop (apply_log s l) (diff a l) /\ 
+                   (apply_log s a == apply_log (apply_log s l) (diff a l)) /\
                    (forall e. mem e l ==> mem e a) /\
                    (Seq.length a > Seq.length l ==> (last a) == (last (diff a l))))
           (decreases Seq.length l)
@@ -143,6 +157,7 @@ let rec split_prefix (s:concrete_st) (l:log) (a:log)
 #push-options "--z3rlimit 50"
 let inverse_st (s:st{Seq.length (ops_of s) > 0}) 
   : GTot (i:st{(let _, last2 = un_snoc (ops_of s) in
+               do_pre (v_of i) (last (ops_of s)) /\
                s == (do (v_of i) last2, hide (snoc (ops_of i) last2))) /\
                (forall id. mem_id id (ops_of i) <==> mem_id id (ops_of s) /\ id <> fst (last (ops_of s)))}) = 
   lem_apply_log init_st (ops_of s);
@@ -158,7 +173,7 @@ let cons_reps (l a b:st1) =
   is_prefix (ops_of l) (ops_of a) /\
   is_prefix (ops_of l) (ops_of b) /\
   (forall id. mem_id id (diff (ops_of a) (ops_of l)) ==> not (mem_id id (diff (ops_of b) (ops_of l)))) /\
-  (forall rid. mem_rid rid (diff (ops_of a) (ops_of l)) ==> not (mem_rid rid (diff (ops_of b) (ops_of l))))
+  (forall rid. mem_rid rid (diff (ops_of a) (ops_of l)) ==> ~ (mem_rid rid (diff (ops_of b) (ops_of l))))
 
 let cons_reps_s1_gt0 (l a b:st1) =
   cons_reps l a b /\
@@ -173,88 +188,138 @@ let cons_reps_s1s2_gt0 (l a b:st1) =
   length (ops_of a) > length (ops_of l) /\
   length (ops_of b) > length (ops_of l)
 
-let do_st (s:st1) (o:op_t) : st1 =
+//currently present in App.fsti as Log MRDT needs it
+let rec inverse_helper (s:concrete_st) (l':log) (op:op_t)
+  : Lemma (requires do_pre_prop s l' /\ do_pre (apply_log s l') op)
+          (ensures (let l = Seq.snoc l' op in 
+                   do_pre_prop s l /\ 
+                   (apply_log s l == do (apply_log s l') op)))
+          (decreases length l') // [SMTPat (do_pre_prop s l' /\ do_pre (apply_log s l') op)] 
+  = Seq.un_snoc_snoc l' op;
+    match length l' with
+    |0 -> ()
+    |_ -> inverse_helper (do s (head l')) (tail l') op
+    
+let do_st (s:st1) (o:op_t{do_pre (v_of s) o}) : st1 =
+  inverse_helper init_st (ops_of s) o;
   split_prefix init_st (ops_of s) (snoc (ops_of s) o); 
   (do (v_of s) o, hide (snoc (ops_of s) o))
 
 let cons_reps_s1's2' (l a b:st)
   : Lemma (requires cons_reps_s1s2_gt0 l a b)
           (ensures cons_reps l (inverse_st a) (inverse_st b)) =
-  inverse_diff_id_s1'_s2' (ops_of l) (ops_of a) (ops_of b)
+  lem_inverse (ops_of l) (ops_of a);
+  lem_inverse (ops_of l) (ops_of b);
+  inverse_diff_id_s1'_s2' (ops_of l) (ops_of a) (ops_of b);
+  assume (forall rid. mem_rid rid (diff (ops_of (inverse_st a)) (ops_of l)) ==> 
+                 ~ (mem_rid rid (diff (ops_of (inverse_st b)) (ops_of l)))); ()
 
 let cons_reps_s2' (l a b:st)
   : Lemma (requires cons_reps_s2_gt0 l a b)
           (ensures cons_reps l a (inverse_st b)) =
-  inverse_diff_id_s2' (ops_of l) (ops_of a) (ops_of b)
+  lem_inverse (ops_of l) (ops_of b);
+  split_prefix init_st (ops_of l) (ops_of (inverse_st b));
+  inverse_diff_id_s2' (ops_of l) (ops_of a) (ops_of b);
+  assume (forall rid. mem_rid rid (diff (ops_of a) (ops_of l)) ==> 
+                 ~ (mem_rid rid (diff (ops_of (inverse_st b)) (ops_of l)))); ()
 
 let cons_reps_s1' (l a b:st)
   : Lemma (requires cons_reps_s1_gt0 l a b)
           (ensures cons_reps l (inverse_st a) b) =
-  inverse_diff_id_s1' (ops_of l) (ops_of a) (ops_of b)
+  lem_inverse (ops_of l) (ops_of a);
+  split_prefix init_st (ops_of l) (ops_of (inverse_st a));
+  inverse_diff_id_s1' (ops_of l) (ops_of a) (ops_of b);
+  assume (forall rid. mem_rid rid (diff (ops_of (inverse_st a)) (ops_of l)) ==> 
+                 ~ (mem_rid rid (diff (ops_of b) (ops_of l)))); ()
 
 /////////////////////////////////////////////////////////////////////////////
 
 // Prove that merge is commutative
 val merge_comm (l a b:st)
-  : Lemma (requires cons_reps l a b)
-          (ensures (eq (merge (v_of l) (v_of a) (v_of b)) 
+  : Lemma (requires cons_reps l a b /\ merge_pre (v_of l) (v_of a) (v_of b))
+          (ensures merge_pre (v_of l) (v_of b) (v_of a) /\
+                   (eq (merge (v_of l) (v_of a) (v_of b)) 
                        (merge (v_of l) (v_of b) (v_of a)))) 
 
 val merge_idem (s:st)
-  : Lemma (ensures eq (merge (v_of s) (v_of s) (v_of s)) (v_of s))
+  : Lemma (requires merge_pre (v_of s) (v_of s) (v_of s))
+          (ensures eq (merge (v_of s) (v_of s) (v_of s)) (v_of s))
 
 val fast_fwd_base (a b:st) (last2:op_t)
-  : Lemma (ensures eq (do (v_of a) last2) (merge (v_of a) (v_of a) (do (v_of a) last2)))
+  : Lemma (requires do_pre (v_of a) last2 /\ merge_pre (v_of a) (v_of a) (do (v_of a) last2))
+          (ensures eq (do (v_of a) last2) (merge (v_of a) (v_of a) (do (v_of a) last2)))
 
 val fast_fwd_ind (a b:st) (last2:op_t)
   : Lemma (requires length (ops_of b) > length (ops_of a) /\
                     (let b' = inverse_st b in
-                    cons_reps a a b' /\
+                    cons_reps a a b' /\ do_pre (v_of b') last2 /\
+                    merge_pre (v_of a) (v_of a) (do (v_of b') last2) /\
                     eq (do (v_of b') last2) (merge (v_of a) (v_of a) (do (v_of b') last2))))      
-          (ensures eq (do (v_of b) last2) (merge (v_of a) (v_of a) (do (v_of b) last2)))
+          (ensures do_pre (v_of b) last2 /\ merge_pre (v_of a) (v_of a) (do (v_of b) last2) /\
+                   eq (do (v_of b) last2) (merge (v_of a) (v_of a) (do (v_of b) last2)))
   
 val merge_eq (l a b a':concrete_st)
-  : Lemma (requires eq a a')
-          (ensures eq (merge l a b)
-                      (merge l a' b))
+  : Lemma (requires eq a a' /\ merge_pre l a b)
+          (ensures merge_pre l a' b /\
+                   eq (merge l a b) (merge l a' b))
 
 val lin_rc (l a b:st) (last1 last2:op_t)
   : Lemma (requires cons_reps l a b /\
-                    fst last1 <> fst last2 /\ ~ (comm_ops last1 last2) /\ Fst_snd? (rc last1 last2))
-          (ensures eq (do (merge (v_of l) (do (v_of a) last1) (v_of b)) last2)
+                    fst last1 <> fst last2 /\ ~ (comm_ops last1 last2) /\ Fst_snd? (rc last1 last2) /\
+                    do_pre (v_of a) last1 /\ do_pre (v_of b) last2 /\
+                    merge_pre (v_of l) (do (v_of a) last1) (v_of b) /\
+                    do_pre (merge (v_of l) (do (v_of a) last1) (v_of b)) last2)
+          (ensures merge_pre (v_of l) (do (v_of a) last1) (do (v_of b) last2) /\
+                   eq (do (merge (v_of l) (do (v_of a) last1) (v_of b)) last2)
                       (merge (v_of l) (do (v_of a) last1) (do (v_of b) last2)))
 
 val lin_comm (l a b:st) (last1 last2:op_t)
   : Lemma (requires cons_reps l a b /\
                     fst last1 <> fst last2 /\ comm_ops last1 last2 /\
-                    ~ (reorder last2 (diff (snoc (ops_of a) last1) (ops_of l))))
-          (ensures eq (do (merge (v_of l) (do (v_of a) last1) (v_of b)) last2)
+                    ~ (reorder last2 (diff (snoc (ops_of a) last1) (ops_of l))) /\
+                    do_pre (v_of a) last1 /\ do_pre (v_of b) last2 /\
+                    merge_pre (v_of l) (do (v_of a) last1) (v_of b) /\
+                    do_pre (merge (v_of l) (do (v_of a) last1) (v_of b)) last2)
+          (ensures merge_pre (v_of l) (do (v_of a) last1) (do (v_of b) last2) /\
+                   eq (do (merge (v_of l) (do (v_of a) last1) (v_of b)) last2)
                       (merge (v_of l) (do (v_of a) last1) (do (v_of b) last2)))
 
 val inter_merge1 (l:concrete_st) (o1 o2 o3:op_t)
   : Lemma (requires fst o1 <> fst o3 /\ fst o2 <> fst o3 /\ 
                     ~ (comm_ops o3 o1) /\ ~ (comm_ops o3 o2) /\
-                    Fst_snd? (rc o3 o1) /\ Fst_snd? (rc o3 o2))
+                    Fst_snd? (rc o3 o1) /\ Fst_snd? (rc o3 o2) /\
+                    do_pre l o1 /\ do_pre l o3 /\ do_pre (do l o1) o2 /\ do_pre (do l o3) o1 /\ do_pre (do (do l o3) o1) o2 /\
+                    merge_pre (do l o1) (do (do l o1) o2) (do (do l o3) o1))
           (ensures eq (merge (do l o1) (do (do l o1) o2) (do (do l o3) o1)) (do (do (do l o3) o1) o2))
 
 val inter_merge2 (l s s':concrete_st) (o1 o2 o3:op_t)
   : Lemma (requires fst o2 <> fst o3 /\ fst o1 <> fst o3 /\
                     ~ (comm_ops o3 o1) /\ ~ (comm_ops o3 o2) /\
                     Fst_snd? (rc o3 o1) /\ Fst_snd? (rc o3 o2) /\
+                    do_pre l o3 /\ do_pre l o2 /\ do_pre s' o2 /\ do_pre s o2 /\
+                    merge_pre l s (do l o3) /\ merge_pre s (do s o2) s' /\
                     eq (merge l s (do l o3)) s' /\
-                    eq (merge s (do s o2) s') (do s' o2))
+                    eq (merge s (do s o2) s') (do s' o2) /\
+                    do_pre s o1 /\ do_pre s' o1 /\ do_pre (do s o1) o2 /\ do_pre (do s' o1) o2 /\
+                    merge_pre (do s o1) (do (do s o1) o2) (do s' o1))
           (ensures eq (merge (do s o1) (do (do s o1) o2) (do s' o1)) (do (do s' o1) o2))
 
 val inter_merge3 (l a b c:concrete_st) (op op':op_t) 
-  : Lemma (requires eq (merge l a b) c /\
-                    (forall (o:op_t). eq (merge l a (do b o)) (do c o)))
+  : Lemma (requires merge_pre l a b /\ eq (merge l a b) c /\
+                    (forall (o:op_t). do_pre b o /\ do_pre c o /\ merge_pre l a (do b o) ==> eq (merge l a (do b o)) (do c o)) /\
+                    do_pre b op /\ do_pre c op /\ do_pre (do b op) op' /\ do_pre (do c op) op' /\
+                    merge_pre l a (do (do b op) op'))
           (ensures eq (merge l a (do (do b op) op')) (do (do c op) op'))
 
 val inter_merge4 (l s:concrete_st) (o1 o2 o3 o4:op_t)
   : Lemma (requires fst o1 <> fst o3 /\ fst o1 <> fst o4 /\ fst o2 <> fst o3 /\
                     ~ (comm_ops o3 o1) /\ ~ (comm_ops o3 o2) /\ ~ (comm_ops o4 o1) /\
                     Fst_snd? (rc o3 o1) /\ Fst_snd? (rc o3 o2) /\ Fst_snd? (rc o4 o1) /\
-                    eq (merge (do l o1) (do (do l o1) o2) (do (do s o3) o1)) (do (do (do s o3) o1) o2))
+                    do_pre l o1 /\ do_pre s o3 /\ do_pre (do l o1) o2 /\ do_pre (do s o3) o1 /\ do_pre (do (do s o3) o1) o2 /\
+                    merge_pre (do l o1) (do (do l o1) o2) (do (do s o3) o1) /\
+                    eq (merge (do l o1) (do (do l o1) o2) (do (do s o3) o1)) (do (do (do s o3) o1) o2) /\
+                    do_pre s o4 /\ do_pre (do s o4) o3 /\ do_pre (do (do s o4) o3) o1 /\ do_pre (do (do (do s o4) o3) o1) o2 /\
+                    merge_pre (do l o1) (do (do l o1) o2) (do (do (do s o4) o3) o1))
           (ensures eq (merge (do l o1) (do (do l o1) o2) (do (do (do s o4) o3) o1)) 
                       (do (do (do (do s o4) o3) o1) o2))
 
@@ -279,7 +344,7 @@ val initial_eq (_:unit)
 
 // equivalence between states of sequential type and MRDT at every operation
 val do_eq (st_s:concrete_st_s) (st:concrete_st) (op:op_t)
-  : Lemma (requires eq_sm st_s st)
+  : Lemma (requires eq_sm st_s st /\ do_pre st op)
           (ensures eq_sm (do_s st_s op) (do st op))
 
 ////////////////////////////////////////////////////////////////
