new/user_rc/2PSet/App_user_rc.fst
@@ -72,6 +72,20 @@ let merge (l a b:concrete_st) : concrete_st =
 
 /////////////////////////////////////////////////////////////////////////////
 
+let no_rc_chain (o1 o2 o3:op_t)
+  : Lemma (requires fst o1 <> fst o2 /\ fst o2 <> fst o3 /\ ~ (comm_ops o1 o2) /\ ~ (comm_ops o2 o3))
+          (ensures ~ (Fst_snd? (rc o1 o2) /\ Fst_snd? (rc o2 o3))) = ()
+
+let relaxed_comm (s:concrete_st) (o1 o2 o3:op_t)
+  : Lemma (requires fst o1 <> fst o2 /\ ~ (comm_ops o1 o2) /\ Fst_snd? (rc o1 o2) /\ ~ (comm_ops o2 o3))
+          (ensures eq (do (do (do s o1) o2) o3) (do (do (do s o2) o1) o3)) = ()
+
+let rc_comm (o1 o2:op_t)
+  : Lemma (requires fst o1 <> fst o2)
+          (ensures ~ (comm_ops o1 o2) ==> (Fst_snd? (rc o1 o2) \/ Fst_snd? (rc o2 o1))) = ()
+
+////////////////////////////////////////////////////////////////////////////
+
 // Prove that merge is commutative
 let merge_comm (l a b:st)
   : Lemma (requires cons_reps l a b)
@@ -114,6 +128,25 @@ let rec lin_rc (l a b:st) (last1 last2:op_t)
      cons_reps_s1' l a b;
      lin_rc l a' b last1 last2)
 
+let cons_reps' (l a b:st1) =
+  distinct_ops (ops_of l) /\ distinct_ops (ops_of a) /\ distinct_ops (ops_of b) /\
+  is_prefix (ops_of l) (ops_of a) /\
+  is_prefix (ops_of l) (ops_of b)
+
+let rec lin_rc' (l a b:st) (last1 last2:op_t)
+  : Lemma (requires cons_reps' l a b /\ 
+                    fst last1 <> fst last2 /\ ~ (comm_ops last1 last2) /\ Fst_snd? (rc last1 last2))
+          (ensures eq (do (merge (v_of l) (do (v_of a) last1) (v_of b)) last2)
+                      (merge (v_of l) (do (v_of a) last1) (do (v_of b) last2)))
+          (decreases %[length (ops_of l); length (ops_of a); length (ops_of b)]) =
+  if ops_of a = ops_of l && ops_of b = ops_of l then ()
+  else if ops_of a = ops_of l then 
+    (let b' = inverse_st b in 
+     lin_rc' l a b' last1 last2)
+  else 
+    (let a' = inverse_st a in
+     lin_rc' l a' b last1 last2)
+     
 let comm_empty_log (x:op_t) (l:log)
   : Lemma (ensures length l = 0 ==> commutative_seq x l) = ()
   
@@ -174,7 +207,29 @@ let rec lin_comm1_r (l a b:st) (last1 last2:op_t)
      un_snoc_snoc (ops_of a') last1';
      un_snoc_snoc (ops_of b) last2;
      not_add_eq l (do_st a' last1') (do_st b last2);
-     lin_comm1_r l a' b last1' last2)       
+     lin_comm1_r l a' b last1' last2)      
+
+let rec lin_comm1_r' (l a b:st) (last1 last2:op_t)
+  : Lemma (requires cons_reps' l a b /\ 
+                    fst last1 <> fst last2 /\ comm_ops last1 last2 /\ Rem? (snd (snd last2)) /\
+                    ~ (reorder last2 (diff (snoc (ops_of a) last1) (ops_of l))))
+          (ensures eq (do (merge (v_of l) (v_of a) (v_of b)) last2)
+                      (merge (v_of l) (v_of a) (do (v_of b) last2)))
+          (decreases %[length (ops_of b); length (ops_of a)]) = 
+  if ops_of a = ops_of l && ops_of b = ops_of l then ()
+  else if ops_of a = ops_of l then
+    (let b' = inverse_st b in
+     lin_comm1_r' l a b' last1 last2)
+  else 
+    (let a' = inverse_st a in
+     let pre1, last1' = un_snoc (ops_of a) in
+     assume (fst last1' <> fst last2);
+     assume (~ (reorder last2 (diff (ops_of a) (ops_of l)))); //can be done
+     un_snoc_snoc (ops_of a') last1';
+     un_snoc_snoc (ops_of b) last2;
+     not_add_eq l (do_st a' last1') (do_st b last2);
+     lin_comm1_r' l a' b last1' last2)      
+     
 #pop-options
 
 let lin_comm (l a b:st) (last1 last2:op_t)
@@ -186,6 +241,15 @@ let lin_comm (l a b:st) (last1 last2:op_t)
   if Rem? (snd (snd last2)) then lin_comm1_r l a b last1 last2
   else ()
                       
+let lin_comm' (l a b:st) (last1 last2:op_t)
+  : Lemma (requires cons_reps' l a b /\
+                    fst last1 <> fst last2 /\ comm_ops last1 last2 /\
+                    ~ (reorder last2 (diff (snoc (ops_of a) last1) (ops_of l))))
+          (ensures eq (do (merge (v_of l) (do (v_of a) last1) (v_of b)) last2)
+                      (merge (v_of l) (do (v_of a) last1) (do (v_of b) last2))) =
+  if Rem? (snd (snd last2)) then lin_comm1_r' l a b last1 last2
+  else ()
+  
 let inter_merge1 (l:concrete_st) (o1 o2 o3:op_t)
   : Lemma (requires fst o1 <> fst o3 /\ fst o2 <> fst o3 /\ 
                     ~ (comm_ops o3 o1) /\ ~ (comm_ops o3 o2) /\
@@ -239,4 +303,188 @@ let do_eq (st_s:concrete_st_s) (st:concrete_st) (op:op_t)
   : Lemma (requires eq_sm st_s st)
           (ensures eq_sm (do_s st_s op) (do st op)) = ()
 
+////////////////////////////////////////////////////////////////
+
+#push-options "--z3rlimit 50 --ifuel 3"
+let prop1 (l:st) (o1 o2:op_t)
+  : Lemma (requires fst o1 <> fst o2 /\ ~ (comm_ops o1 o2) /\ Fst_snd? (rc o2 o1))
+          (ensures eq (merge (do (v_of l) o1) (do (v_of l) o1) (do (do (v_of l) o2) o1))
+                      (do (do (v_of l) o2) o1)) = ()
+
+let prop2 (l:st) (o1 o2:op_t) (l2:log)
+  : Lemma (requires fst o1 <> fst o2 /\ ~ (comm_ops o1 o2) /\ Fst_snd? (rc o2 o1))
+          (ensures eq (merge (do (v_of l) o1) (do (v_of l) o1) (apply_log (do (do (v_of l) o2) o1) l2))
+                      (apply_log (do (do (v_of l) o2) o1) l2)) = admit() //fast fwd case
+
+let prop3 (l:st) (o1 o2:op_t) (l1:log)
+  : Lemma (requires fst o1 <> fst o2 /\ ~ (comm_ops o1 o2) /\ Fst_snd? (rc o2 o1) /\
+                    not (mem_id (fst o1) l1))
+          (ensures eq (merge (do (v_of l) o1) (apply_log (do (v_of l) o1) l1) (do (do (v_of l) o2) o1))
+                      (apply_log (do (do (v_of l) o2) o1) l1)) = admit() //!!! 4 suf cond will handle this case
+
+let rec prop3_base_rc (l:st) (o1 o2:op_t) (last1 last2:op_t)
+  : Lemma (requires fst o1 <> fst o2 /\ ~ (comm_ops o1 o2) /\ Fst_snd? (rc o2 o1) /\
+                    fst last1 <> fst last2 /\ ~ (comm_ops last1 last2) /\ Fst_snd? (rc last1 last2) /\
+                    comm_ops o1 last1 /\ not (mem_id (fst last2) (ops_of l)))
+          (ensures eq (merge (do (v_of l) o1) (do (do (v_of l) o1) last1) (do (do (do (v_of l) o2) o1) last2))
+                      (do (merge (do (v_of l) o1) (do (do (v_of l) o1) last1) (do (do (v_of l) o2) o1)) last2))
+          (decreases length (ops_of l)) =
+  if length (ops_of l) = 0 then ()
+  else 
+    (let l' = inverse_st l in
+     let pre, lastl = un_snoc (ops_of l) in
+     lem_last (ops_of l);
+       //assert (fst lastl <> fst last2);
+     prop3_base_rc l' o1 o2 last1 last2)
+
+let prop4_base_comm (l:st) (o1 o2:op_t) (last1 last2:op_t)
+  : Lemma (requires fst o1 <> fst o2 /\ ~ (comm_ops o1 o2) /\ Fst_snd? (rc o2 o1) /\ comm_ops last1 o1 /\
+                    fst last1 <> fst last2 /\ comm_ops last1 last2 /\ not (reorder last2 (create 1 last1)))
+          (ensures eq (merge (do (v_of l) o1) (do (do (v_of l) o1) last1) (do (do (do (v_of l) o2) o1) last2))
+                      (do (merge (do (v_of l) o1) (do (do (v_of l) o1) last1) (do (do (v_of l) o2) o1)) last2)) = ()
+
+let prop3_ind_rc1 (l:concrete_st) (o1 o2:op_t) (l1' l2':log) (last1 last2:op_t)
+  : Lemma (requires fst o1 <> fst o2 /\ ~ (comm_ops o1 o2) /\ Fst_snd? (rc o2 o1) /\ 
+                    fst last1 <> fst last2 /\ ~ (comm_ops last1 last2) /\ Fst_snd? (rc last1 last2) /\
+                    length l2' > 0 /\ 
+                    (let pre2, lastl2 = un_snoc l2' in
+                     eq (merge (do l o1) (do (apply_log (do l o1) l1') last1) (do (apply_log (do (do l o2) o1) pre2) last2))
+                        (do (merge (do l o1) (do (apply_log (do l o1) l1') last1) (apply_log (do (do l o2) o1) pre2)) last2)))
+          (ensures eq (merge (do l o1) (do (apply_log (do l o1) l1') last1) (do (apply_log (do (do l o2) o1) l2') last2))
+                      (do (merge (do l o1) (do (apply_log (do l o1) l1') last1) (apply_log (do (do l o2) o1) l2')) last2)) = ()
+
+let prop3_ind_rc2 (l:concrete_st) (o1 o2:op_t) (l1' l2':log) (last1 last2:op_t)
+  : Lemma (requires fst o1 <> fst o2 /\ ~ (comm_ops o1 o2) /\ Fst_snd? (rc o2 o1) /\
+                    fst last1 <> fst last2 /\ ~ (comm_ops last1 last2) /\ Fst_snd? (rc last1 last2) /\
+                    length l2' = 0 /\ length l1' > 0 /\
+                    (let pre1, lastl1 = un_snoc l1' in
+                     eq (merge (do l o1) (do (apply_log (do l o1) pre1) last1) (do (apply_log (do (do l o2) o1) l2') last2))
+                        (do (merge (do l o1) (do (apply_log (do l o1) pre1) last1) (apply_log (do (do l o2) o1) l2')) last2)))
+          (ensures eq (merge (do l o1) (do (apply_log (do l o1) l1') last1) (do (apply_log (do (do l o2) o1) l2') last2))
+                      (do (merge (do l o1) (do (apply_log (do l o1) l1') last1) (apply_log (do (do l o2) o1) l2')) last2)) = ()
+
+let prop4_ind_comm1 (l:concrete_st) (o1 o2:op_t) (l1' l2':log) (last1 last2:op_t)
+  : Lemma (requires fst o1 <> fst o2 /\ ~ (comm_ops o1 o2) /\ Fst_snd? (rc o2 o1) /\ comm_ops o1 last1 /\
+                    fst last1 <> fst last2 /\ comm_ops last1 last2 /\
+                    //~ (reorder last2 l1') /\
+                    length l2' > 0 /\
+                    (let pre2, lastl2 = un_snoc l2' in
+                     eq (merge (do l o1) (do (apply_log (do l o1) l1') last1) (do (apply_log (do (do l o2) o1) pre2) last2))
+                        (do (merge (do l o1) (do (apply_log (do l o1) l1') last1) (apply_log (do (do l o2) o1) pre2)) last2)))
+          (ensures eq (merge (do l o1) (do (apply_log (do l o1) l1') last1) (do (apply_log (do (do l o2) o1) l2') last2))
+                      (do (merge (do l o1) (do (apply_log (do l o1) l1') last1) (apply_log (do (do l o2) o1) l2')) last2)) = 
+  let pre2, lastl2 = un_snoc l2' in
+  assume (apply_log (do (do l o2) o1) l2' == do (apply_log (do (do l o2) o1) pre2) lastl2); //can be done
+  ()
+
+let prop4_ind_comm2 (l:concrete_st) (o1 o2:op_t) (l1' l2':log) (last1 last2:op_t)
+  : Lemma (requires fst o1 <> fst o2 /\ ~ (comm_ops o1 o2) /\ Fst_snd? (rc o2 o1) /\ comm_ops o1 last1 /\
+                    fst last1 <> fst last2 /\ comm_ops last1 last2 /\
+                    ~ (reorder last2 l1') /\
+                    length l2' = 0 /\ length l1' > 0 /\
+                    (let pre1, lastl1 = un_snoc l1' in
+                     eq (merge (do l o1) (do (apply_log (do l o1) pre1) last1) (do (apply_log (do (do l o2) o1) l2') last2))
+                        (do (merge (do l o1) (do (apply_log (do l o1) pre1) last1) (apply_log (do (do l o2) o1) l2')) last2)))
+          (ensures eq (merge (do l o1) (do (apply_log (do l o1) l1') last1) (do (apply_log (do (do l o2) o1) l2') last2))
+                      (do (merge (do l o1) (do (apply_log (do l o1) l1') last1) (apply_log (do (do l o2) o1) l2')) last2)) = 
+  let pre1, lastl1 = un_snoc l1' in
+  assume (apply_log (do l o1) l1' == do (apply_log (do l o1) pre1) lastl1); //can be done
+  assume (Rem? (snd (snd last2)) ==> ~ (Add? (snd (snd lastl1)) /\ get_ele last2 = get_ele lastl1)); //can be inferred from ~ (reorder last2 l1')
+  ()
+                      
+
+(*
+let rec prop2 (l:st) (o1 o2:op_t) (l2:log)
+  : Lemma (requires fst o1 <> fst o2 /\ ~ (comm_ops o1 o2) /\ Fst_snd? (rc o2 o1))
+          (ensures eq (merge (do (v_of l) o1) (do (v_of l) o1) (apply_log (do (do (v_of l) o2) o1) l2))
+                      (apply_log (do (do (v_of l) o2) o1) l2))
+          (decreases length l2) =
+  if length l2 = 0 then ()
+  else 
+    (let pre2,last2 = un_snoc l2 in
+     assume (apply_log (do (do (v_of l) o2) o1) l2 == do (apply_log (do (do (v_of l) o2) o1) pre2) last2); //can be done
+     prop2 l o1 o2 pre2)
+
+let prop4_ind_comm2' (l:concrete_st) (o1 o2:op_t) (l1' l2':log) (last1 last2:op_t)
+  : Lemma (requires fst o1 <> fst o2 /\ ~ (comm_ops o1 o2) /\ Fst_snd? (rc o2 o1) /\ comm_ops o1 last1 /\
+                    fst last1 <> fst last2 /\ comm_ops last1 last2 /\
+                    length l2' = 0 /\ length l1' > 0 /\
+                    (let pre1, lastl1 = un_snoc l1' in
+                     eq (merge (do l o1) (apply_log (do l o1) l1') (do (apply_log (do (do l o2) o1) l2') last2))
+                        (do (merge (do l o1) (apply_log (do l o1) l1') (apply_log (do (do l o2) o1) l2')) last2)))
+          (ensures eq (merge (do l o1) (do (apply_log (do l o1) l1') last1) (do (apply_log (do (do l o2) o1) l2') last2))
+                      (do (merge (do l o1) (do (apply_log (do l o1) l1') last1) (apply_log (do (do l o2) o1) l2')) last2)) = ()
+
+let rec prop3_base_rc (l:st) (o1 o2:op_t) (last1 last2:op_t)
+  : Lemma (requires fst o1 <> fst o2 /\ ~ (comm_ops o1 o2) /\ Fst_snd? (rc o2 o1) /\
+                    fst last1 <> fst last2 /\ ~ (comm_ops last1 last2) /\ Fst_snd? (rc last1 last2) /\
+                    not (mem_id (fst last2) (ops_of l)))
+          (ensures eq (merge (v_of l) (do (do (v_of l) o1) last1) (do (do (do (v_of l) o2) o1) last2))
+                      (do (merge (v_of l) (do (do (v_of l) o1) last1) (do (do (v_of l) o2) o1)) last2))
+          (decreases length (ops_of l)) =
+  if length (ops_of l) = 0 then ()
+  else 
+    (let l' = inverse_st l in
+     let pre, lastl = un_snoc (ops_of l) in
+     lem_last (ops_of l);
+       //assert (fst lastl <> fst last2);
+     prop3_base_rc l' o1 o2 last1 last2)
+
+let prop4_base_comm (l:st) (o1 o2:op_t) (last1 last2:op_t)
+  : Lemma (requires fst o1 <> fst o2 /\ ~ (comm_ops o1 o2) /\ Fst_snd? (rc o2 o1) /\ comm_ops last1 o1 /\
+                    fst last1 <> fst last2 /\ comm_ops last1 last2 /\ not (reorder last2 (create 1 last1)))
+          (ensures eq (merge (v_of l) (do (do (v_of l) o1) last1) (do (do (do (v_of l) o2) o1) last2))
+                      (do (merge (v_of l) (do (do (v_of l) o1) last1) (do (do (v_of l) o2) o1)) last2)) = ()
+
+let prop3_ind_rc1 (l:concrete_st) (o1 o2:op_t) (l1' l2':log) (last1 last2:op_t)
+  : Lemma (requires fst o1 <> fst o2 /\ ~ (comm_ops o1 o2) /\ Fst_snd? (rc o2 o1) /\
+                    fst last1 <> fst last2 /\ ~ (comm_ops last1 last2) /\ Fst_snd? (rc last1 last2) /\
+                    length l2' > 0 /\ 
+                    (let pre2, lastl2 = un_snoc l2' in
+                     eq (merge l (do (apply_log (do l o1) l1') last1) (do (apply_log (do (do l o2) o1) pre2) last2))
+                        (do (merge l (do (apply_log (do l o1) l1') last1) (apply_log (do (do l o2) o1) pre2)) last2)))
+          (ensures eq (merge l (do (apply_log (do l o1) l1') last1) (do (apply_log (do (do l o2) o1) l2') last2))
+                      (do (merge l (do (apply_log (do l o1) l1') last1) (apply_log (do (do l o2) o1) l2')) last2)) = ()
+
+let prop3_ind_rc2 (l:concrete_st) (o1 o2:op_t) (l1' l2':log) (last1 last2:op_t)
+  : Lemma (requires fst o1 <> fst o2 /\ ~ (comm_ops o1 o2) /\ Fst_snd? (rc o2 o1) /\
+                    fst last1 <> fst last2 /\ ~ (comm_ops last1 last2) /\ Fst_snd? (rc last1 last2) /\
+                    length l2' = 0 /\ length l1' > 0 /\
+                    (let pre1, lastl1 = un_snoc l1' in
+                     eq (merge l (do (apply_log (do l o1) pre1) last1) (do (apply_log (do (do l o2) o1) l2') last2))
+                        (do (merge l (do (apply_log (do l o1) pre1) last1) (apply_log (do (do l o2) o1) l2')) last2)))
+          (ensures eq (merge l (do (apply_log (do l o1) l1') last1) (do (apply_log (do (do l o2) o1) l2') last2))
+                      (do (merge l (do (apply_log (do l o1) l1') last1) (apply_log (do (do l o2) o1) l2')) last2)) = ()
+
+let prop4_ind_comm1 (l:concrete_st) (o1 o2:op_t) (l1' l2':log) (last1 last2:op_t)
+  : Lemma (requires fst o1 <> fst o2 /\ ~ (comm_ops o1 o2) /\ Fst_snd? (rc o2 o1) /\ comm_ops o1 last1 /\
+                    fst last1 <> fst last2 /\ comm_ops last1 last2 /\
+                    length l2' > 0 /\
+                    (let pre2, lastl2 = un_snoc l2' in
+                     fst lastl2 <> fst o1 /\
+                     eq (merge l (do (apply_log (do l o1) l1') last1) (do (apply_log (do (do l o2) o1) pre2) last2))
+                        (do (merge l (do (apply_log (do l o1) l1') last1) (apply_log (do (do l o2) o1) pre2)) last2)))
+          (ensures eq (merge l (do (apply_log (do l o1) l1') last1) (do (apply_log (do (do l o2) o1) l2') last2))
+                      (do (merge l (do (apply_log (do l o1) l1') last1) (apply_log (do (do l o2) o1) l2')) last2)) = admit()
+
+(*let prop4_ind_comm1' (l:concrete_st) (o1 o2:op_t) (l1' l2':log) (last1 last2:op_t)
+  : Lemma (requires fst o1 <> fst o2 /\ ~ (comm_ops o1 o2) /\ Fst_snd? (rc o2 o1) /\ comm_ops o1 last1 /\
+                    fst last1 <> fst last2 /\ comm_ops last1 last2 /\
+                    length l1' > 0 /\ 
+                    (let pre1, lastl1 = un_snoc l1' in
+                     eq (merge l (apply_log (do l o1) l1') (do (apply_log (do (do l o2) o1) l2') last2))
+                        (do (merge l (apply_log (do l o1) l1') (apply_log (do (do l o2) o1) l2')) last2)))
+          (ensures eq (merge l (do (apply_log (do l o1) l1') last1) (do (apply_log (do (do l o2) o1) l2') last2))
+                      (do (merge l (do (apply_log (do l o1) l1') last1) (apply_log (do (do l o2) o1) l2')) last2)) = ()*)
+                      
+let prop4_ind_comm2 (l:concrete_st) (o1 o2:op_t) (l1' l2':log) (last1 last2:op_t)
+  : Lemma (requires fst o1 <> fst o2 /\ ~ (comm_ops o1 o2) /\ Fst_snd? (rc o2 o1) /\ comm_ops o1 last1 /\
+                    fst last1 <> fst last2 /\ comm_ops last1 last2 /\
+                    length l2' = 0 /\ length l1' > 0 /\
+                    (let pre1, lastl1 = un_snoc l1' in
+                     eq (merge l (apply_log (do l o1) l1') (do (apply_log (do (do l o2) o1) l2') last2))
+                        (do (merge l (apply_log (do l o1) l1') (apply_log (do (do l o2) o1) l2')) last2)))
+          (ensures eq (merge l (do (apply_log (do l o1) l1') last1) (do (apply_log (do (do l o2) o1) l2') last2))
+                      (do (merge l (do (apply_log (do l o1) l1') last1) (apply_log (do (do l o2) o1) l2')) last2)) = ()*)
+                      
 ////////////////////////////////////////////////////////////////
