new/user_rc/Enable-wins_flag/App_user_rc.fst
@@ -83,7 +83,46 @@ let merge (l a b:concrete_st) : concrete_st =
   let keys = S.union (M.domain l) (S.union (M.domain a) (M.domain b)) in
   let u = M.const_on keys (0, false) in
   M.iter_upd (fun k v -> merge_cf (sel l k) (sel a k) (sel b k)) u
+  
+/////////////////////////////////////////////////////////////////////////////
 
+let no_rc_chain (o1 o2 o3:op_t)
+  : Lemma (requires fst o1 <> fst o2 /\ fst o2 <> fst o3 /\ ~ (comm_ops o1 o2) /\ ~ (comm_ops o2 o3))
+          (ensures ~ (Fst_snd? (rc o1 o2) /\ Fst_snd? (rc o2 o3))) = ()
+
+let relaxed_comm (s:concrete_st) (o1 o2 o3:op_t)
+  : Lemma (requires fst o1 <> fst o2 /\ ~ (comm_ops o1 o2) /\ Fst_snd? (rc o1 o2) /\ ~ (comm_ops o2 o3))
+          (ensures eq (do (do (do s o1) o2) o3) (do (do (do s o2) o1) o3)) = ()
+
+let rc_comm (o1 o2:op_t)
+  : Lemma (requires fst o1 <> fst o2)
+          (ensures ~ (comm_ops o1 o2) ==> (Fst_snd? (rc o1 o2) \/ Fst_snd? (rc o2 o1))) = ()
+
+let base (l:concrete_st) (o1 o2:op_t)
+  : Lemma (requires fst o1 <> fst o2 /\ ~ (comm_ops o1 o2) /\ Fst_snd? (rc o2 o1))
+          (ensures eq (merge l (do l o1) (do l o2)) (do (do l o2) o1)) = ()
+
+#push-options "--z3rlimit 50 --ifuel 3 --split_queries always"
+let rec trial (l:st) (o1 o2:op_t) (l1 l2:log)
+  : Lemma (requires distinct_ops l1 /\ distinct_ops l2 /\ (forall id1 id2. mem_id id1 l1 ==> not (mem_id id2 l2)) /\
+                    not (mem_id (fst o1) l1) /\ not (mem_id (fst o1) l2) /\
+                    not (mem_id (fst o2) l1) /\ not (mem_id (fst o2) l2) /\
+                    fst o1 <> fst o2 /\ ~ (comm_ops o1 o2) /\ Fst_snd? (rc o2 o1))
+          (ensures true)
+          (decreases %[length l1; length l2]) =
+  if length l1 = 0 && length l2 = 0 then 
+    (assert (eq (merge (v_of l) (do (v_of l) o1) (do (v_of l) o2)) (do (do (v_of l) o2) o1)); ())
+  else if length l2 = 0 then
+    (let pre, last1 = un_snoc l1 in
+     assume (distinct_ops pre /\ (forall id1 id2. mem_id id1 pre ==> not (mem_id id2 l2)) /\
+             not (mem_id (fst o1) pre) /\ not (mem_id (fst o2) pre) /\ not (mem_id (fst o2) l2));
+     trial l o1 o2 pre l2; 
+     assume (apply_log (do (v_of l) o1) l1 = do (apply_log (do (v_of l) o1) pre) last1);
+     assume (apply_log (do (do (v_of l) o2) o1) l1 = do (apply_log (do (do (v_of l) o2) o1) pre) last1);
+     assert (eq (merge (v_of l) (apply_log (do (v_of l) o1) l1) (do (do (v_of l) o2) o1))
+                (apply_log (do (do (v_of l) o2) o1) l1)); ())
+  else ()
+  
 
 /////////////////////////////////////////////////////////////////////////////
 
@@ -164,6 +203,34 @@ let rec lin_rc (l a b:st) (last1 last2:op_t)
      lin_rc l a' b last1 last2;
      lin_rc_ind_a' l a b last1 last2)
 
+let lin_rc_a' (l a b:st) (last1 last2:op_t)
+  : Lemma (requires cons_reps l a b /\ 
+                    fst last1 <> fst last2 /\ ~ (comm_ops last1 last2) /\ Snd_fst? (rc last1 last2))
+          (ensures eq (do (merge (v_of l) (v_of a) (do (v_of b) last2)) last1)
+                      (merge (v_of l) (do (v_of a) last1) (do (v_of b) last2))) =
+  lin_rc l b a last2 last1
+                      
+let cons_reps' (l a b:st1) =
+  distinct_ops (ops_of l) /\ distinct_ops (ops_of a) /\ distinct_ops (ops_of b) /\
+  is_prefix (ops_of l) (ops_of a) /\
+  is_prefix (ops_of l) (ops_of b)
+
+let rec lin_rc' (l a b:st) (last1 last2:op_t)
+  : Lemma (requires cons_reps' l a b /\ 
+                    fst last1 <> fst last2 /\ ~ (comm_ops last1 last2) /\ Fst_snd? (rc last1 last2))
+          (ensures eq (do (merge (v_of l) (do (v_of a) last1) (v_of b)) last2)
+                      (merge (v_of l) (do (v_of a) last1) (do (v_of b) last2)))
+          (decreases %[length (ops_of a); length (ops_of b)]) =
+  if ops_of a = ops_of l && ops_of b = ops_of l then ()
+  else if ops_of a = ops_of l then 
+    (let b' = inverse_st b in 
+     lin_rc' l a b' last1 last2;
+     lin_rc_ind_b' l a b last1 last2) 
+  else 
+    (let a' = inverse_st a in
+     lin_rc' l a' b last1 last2;
+     lin_rc_ind_a' l a b last1 last2)
+     
 let lin_comm_ind_b' (l a b:st) (last1 last2:op_t)
   : Lemma (requires length (ops_of b) > length (ops_of l) /\
                     comm_ops last1 last2 /\
@@ -204,6 +271,24 @@ let rec lin_comm1 (l a b:st) (last1 last2:op_t)
      cons_reps_s2' l a b;
      lin_comm1 l a b' last1 last2;
      lin_comm_ind_b' l a b last1 last2)
+
+let rec lin_comm1' (l a b:st) (last1 last2:op_t)
+  : Lemma (requires cons_reps' l a b /\
+                    fst last1 <> fst last2 /\ comm_ops last1 last2)
+                    //~ (reorder last2 (diff (snoc (ops_of a) last1) (ops_of l))))
+          (ensures eq (do (merge (v_of l) (do (v_of a) last1) (v_of b)) last2)
+                      (merge (v_of l) (do (v_of a) last1) (do (v_of b) last2)))
+          (decreases %[length (ops_of a); length (ops_of b)]) = 
+  if ops_of a = ops_of l && ops_of b = ops_of l then ()
+  else if ops_of b = ops_of l then 
+    (let a' = inverse_st a in
+     lin_comm1' l a' b last1 last2;
+     lin_comm_ind_a' l a b last1 last2)
+  else 
+    (let b' = inverse_st b in
+     lin_comm1' l a b' last1 last2;
+     lin_comm_ind_b' l a b last1 last2)
+     
 #pop-options
 
 let lin_comm (l a b:st) (last1 last2:op_t)
@@ -213,17 +298,25 @@ let lin_comm (l a b:st) (last1 last2:op_t)
           (ensures eq (do (merge (v_of l) (do (v_of a) last1) (v_of b)) last2)
                       (merge (v_of l) (do (v_of a) last1) (do (v_of b) last2))) =
   lin_comm1 l a b last1 last2
-                      
+
+let lin_comm' (l a b:st) (last1 last2:op_t)
+  : Lemma (requires cons_reps' l a b /\
+                    fst last1 <> fst last2 /\ comm_ops last1 last2 /\
+                    ~ (reorder last2 (diff (snoc (ops_of a) last1) (ops_of l))))
+          (ensures eq (do (merge (v_of l) (do (v_of a) last1) (v_of b)) last2)
+                      (merge (v_of l) (do (v_of a) last1) (do (v_of b) last2))) =
+  lin_comm1' l a b last1 last2
+  
 let inter_merge1 (l:concrete_st) (o1 o2 o3:op_t)
   : Lemma (requires fst o1 <> fst o3 /\ fst o2 <> fst o3 /\ 
                     ~ (comm_ops o3 o1) /\ ~ (comm_ops o3 o2) /\
-                    Fst_snd? (rc o3 o1) /\ Fst_snd? (rc o3 o2))
+                    Fst_snd? (rc o3 o1) (*/\ Fst_snd? (rc o3 o2*))
           (ensures eq (merge (do l o1) (do (do l o1) o2) (do (do l o3) o1)) (do (do (do l o3) o1) o2)) = ()
 
 let inter_merge2 (l s s':concrete_st) (o1 o2 o3:op_t)
   : Lemma (requires fst o2 <> fst o3 /\ fst o1 <> fst o3 /\
                     ~ (comm_ops o3 o1) /\ ~ (comm_ops o3 o2) /\
-                    Fst_snd? (rc o3 o1) /\ Fst_snd? (rc o3 o2) /\
+                    Fst_snd? (rc o3 o1) /\ //Fst_snd? (rc o3 o2) /\
                     eq (merge l s (do l o3)) s' /\
                     eq (merge s (do s o2) s') (do s' o2))
           (ensures eq (merge (do s o1) (do (do s o1) o2) (do s' o1)) (do (do s' o1) o2)) = ()
@@ -238,7 +331,7 @@ let inter_merge3 (l a b c:concrete_st) (op op':op_t)
 let inter_merge4 (l s:concrete_st) (o1 o2 o3 o4:op_t)
   : Lemma (requires fst o1 <> fst o3 /\ fst o1 <> fst o4 /\ fst o2 <> fst o3 /\
                     ~ (comm_ops o3 o1) /\ ~ (comm_ops o3 o2) /\ ~ (comm_ops o4 o1) /\
-                    Fst_snd? (rc o3 o1) /\ Fst_snd? (rc o3 o2) /\ Fst_snd? (rc o4 o1) /\
+                    Fst_snd? (rc o3 o1) /\ //Fst_snd? (rc o3 o2) /\ Fst_snd? (rc o4 o1) /\
                     eq (merge (do l o1) (do (do l o1) o2) (do (do s o3) o1)) (do (do (do s o3) o1) o2))
           (ensures eq (merge (do l o1) (do (do l o1) o2) (do (do (do s o4) o3) o1)) 
                       (do (do (do (do s o4) o3) o1) o2)) = ()
@@ -271,4 +364,165 @@ let do_eq (st_s:concrete_st_s) (st:concrete_st) (op:op_t)
   : Lemma (requires eq_sm st_s st)
           (ensures eq_sm (do_s st_s op) (do st op)) = ()
 
+////////////////////////////////////////////////////////////////
+
+#push-options "--z3rlimit 50 --ifuel 3"
+let prop1 (l:st) (o1 o2:op_t)
+  : Lemma (requires fst o1 <> fst o2 /\ ~ (comm_ops o1 o2) /\ Fst_snd? (rc o2 o1))
+          (ensures eq (merge (do (v_of l) o1) (do (v_of l) o1) (do (do (v_of l) o2) o1))
+                      (do (do (v_of l) o2) o1)) = ()
+
+let prop2 (l:st) (o1 o2:op_t) (l2:log)
+  : Lemma (requires fst o1 <> fst o2 /\ ~ (comm_ops o1 o2) /\ Fst_snd? (rc o2 o1) /\ get_rid o1 <> get_rid o2)
+          (ensures eq (merge (do (v_of l) o1) (do (v_of l) o1) (apply_log (do (do (v_of l) o2) o1) l2))
+                      (apply_log (do (do (v_of l) o2) o1) l2)) = admit() //fast fwd case, already proven
+
+let prop3 (l:st) (o1 o2:op_t) (l1:log)
+  : Lemma (requires fst o1 <> fst o2 /\ ~ (comm_ops o1 o2) /\ Fst_snd? (rc o2 o1))
+          (ensures eq (merge (do (v_of l) o1) (apply_log (do (v_of l) o1) l1) (do (do (v_of l) o2) o1))
+                      (apply_log (do (do (v_of l) o2) o1) l1)) = admit() //!!! 4 suf cond will handle this case
+                      
+let rec prop3_base_rc (l:st) (o1 o2:op_t) (last1 last2:op_t)
+  : Lemma (requires fst o1 <> fst o2 /\ ~ (comm_ops o1 o2) /\ Fst_snd? (rc o2 o1) /\
+                    fst last1 <> fst last2 /\ ~ (comm_ops last1 last2) /\ Fst_snd? (rc last1 last2) /\
+                    comm_ops o1 last1 /\ not (mem_id (fst last2) (ops_of l)))
+          (ensures eq (merge (do (v_of l) o1) (do (do (v_of l) o1) last1) (do (do (do (v_of l) o2) o1) last2))
+                      (do (merge (do (v_of l) o1) (do (do (v_of l) o1) last1) (do (do (v_of l) o2) o1)) last2))
+          (decreases length (ops_of l)) =
+  if length (ops_of l) = 0 then ()
+  else prop3_base_rc (inverse_st l) o1 o2 last1 last2
+
+let prop4_base_comm (l:st) (o1 o2:op_t) (last1 last2:op_t)
+  : Lemma (requires fst o1 <> fst o2 /\ ~ (comm_ops o1 o2) /\ Fst_snd? (rc o2 o1) /\ comm_ops last1 o1 /\
+                    fst last1 <> fst last2 /\ comm_ops last1 last2 /\ not (reorder last2 (create 1 last1)))
+          (ensures eq (merge (do (v_of l) o1) (do (do (v_of l) o1) last1) (do (do (do (v_of l) o2) o1) last2))
+                      (do (merge (do (v_of l) o1) (do (do (v_of l) o1) last1) (do (do (v_of l) o2) o1)) last2)) = ()
+
+let prop3_ind_rc1 (l:concrete_st) (o1 o2:op_t) (l1' l2':log) (last1 last2:op_t)
+  : Lemma (requires fst o1 <> fst o2 /\ ~ (comm_ops o1 o2) /\ Fst_snd? (rc o2 o1) /\ comm_ops o1 last1 /\
+                    fst last1 <> fst last2 /\ ~ (comm_ops last1 last2) /\ Fst_snd? (rc last1 last2) /\
+                    length l2' > 0 /\ 
+                    (let pre2, lastl2 = un_snoc l2' in
+                     eq (merge (do l o1) (do (apply_log (do l o1) l1') last1) (do (apply_log (do (do l o2) o1) pre2) last2))
+                        (do (merge (do l o1) (do (apply_log (do l o1) l1') last1) (apply_log (do (do l o2) o1) pre2)) last2)))
+          (ensures eq (merge (do l o1) (do (apply_log (do l o1) l1') last1) (do (apply_log (do (do l o2) o1) l2') last2))
+                      (do (merge (do l o1) (do (apply_log (do l o1) l1') last1) (apply_log (do (do l o2) o1) l2')) last2)) = ()
+
+let prop3_ind_rc2 (l:concrete_st) (o1 o2:op_t) (l1' l2':log) (last1 last2:op_t)
+  : Lemma (requires fst o1 <> fst o2 /\ ~ (comm_ops o1 o2) /\ Fst_snd? (rc o2 o1) /\
+                    fst last1 <> fst last2 /\ ~ (comm_ops last1 last2) /\ Fst_snd? (rc last1 last2) /\
+                    length l2' = 0 /\ length l1' > 0 /\
+                    (let pre1, lastl1 = un_snoc l1' in
+                     eq (merge (do l o1) (do (apply_log (do l o1) pre1) last1) (do (apply_log (do (do l o2) o1) l2') last2))
+                        (do (merge (do l o1) (do (apply_log (do l o1) pre1) last1) (apply_log (do (do l o2) o1) l2')) last2)))
+          (ensures eq (merge (do l o1) (do (apply_log (do l o1) l1') last1) (do (apply_log (do (do l o2) o1) l2') last2))
+                      (do (merge (do l o1) (do (apply_log (do l o1) l1') last1) (apply_log (do (do l o2) o1) l2')) last2)) = ()
+
+let prop4_ind_comm1 (l:concrete_st) (o1 o2:op_t) (l1' l2':log) (last1 last2:op_t)
+  : Lemma (requires fst o1 <> fst o2 /\ ~ (comm_ops o1 o2) /\ Fst_snd? (rc o2 o1) /\ comm_ops o1 last1 /\
+                    fst last1 <> fst last2 /\ comm_ops last1 last2 /\
+                    //~ (reorder last2 l1') /\
+                    length l2' > 0 /\
+                    (let pre2, lastl2 = un_snoc l2' in
+                     eq (merge (do l o1) (do (apply_log (do l o1) l1') last1) (do (apply_log (do (do l o2) o1) pre2) last2))
+                        (do (merge (do l o1) (do (apply_log (do l o1) l1') last1) (apply_log (do (do l o2) o1) pre2)) last2)))
+          (ensures eq (merge (do l o1) (do (apply_log (do l o1) l1') last1) (do (apply_log (do (do l o2) o1) l2') last2))
+                      (do (merge (do l o1) (do (apply_log (do l o1) l1') last1) (apply_log (do (do l o2) o1) l2')) last2)) = 
+  let pre2, lastl2 = un_snoc l2' in
+  assume (apply_log (do (do l o2) o1) l2' == do (apply_log (do (do l o2) o1) pre2) lastl2); //can be done
+  ()
+
+let prop4_ind_comm2 (l:concrete_st) (o1 o2:op_t) (l1' l2':log) (last1 last2:op_t)
+  : Lemma (requires fst o1 <> fst o2 /\ ~ (comm_ops o1 o2) /\ Fst_snd? (rc o2 o1) /\ comm_ops o1 last1 /\
+                    fst last1 <> fst last2 /\ comm_ops last1 last2 /\
+                    //~ (reorder last2 l1') /\
+                    length l2' = 0 /\ length l1' > 0 /\
+                    (let pre1, lastl1 = un_snoc l1' in
+                     eq (merge (do l o1) (do (apply_log (do l o1) pre1) last1) (do (apply_log (do (do l o2) o1) l2') last2))
+                        (do (merge (do l o1) (do (apply_log (do l o1) pre1) last1) (apply_log (do (do l o2) o1) l2')) last2)))
+          (ensures eq (merge (do l o1) (do (apply_log (do l o1) l1') last1) (do (apply_log (do (do l o2) o1) l2') last2))
+                      (do (merge (do l o1) (do (apply_log (do l o1) l1') last1) (apply_log (do (do l o2) o1) l2')) last2)) = ()
+                      
+////////////////////////////////////////////////////////////////
+
+(*
+let rec prop3 (l:st) (o1 o2:op_t) (l1:log)
+  : Lemma (requires fst o1 <> fst o2 /\ ~ (comm_ops o1 o2) /\ Fst_snd? (rc o2 o1))
+          (ensures eq (merge (do (v_of l) o1) (apply_log (do (v_of l) o1) l1) (do (do (v_of l) o2) o1))
+                      (apply_log (do (do (v_of l) o2) o1) l1)) 
+          (decreases length l1) =
+  if length l1 = 0 then ()
+  else 
+    (let pre1, last1 = un_snoc l1 in
+     assume (get_rid last1 = get_rid o1); //is it true?????
+     assume (apply_log (do (v_of l) o1) l1 == do (apply_log (do (v_of l) o1) pre1) last1); //can be done
+     assume (apply_log (do (do (v_of l) o2) o1) l1 == do (apply_log (do (do (v_of l) o2) o1) pre1) last1); //can be done
+     prop3 l o1 o2 pre1)
+
+let prop4_ind_comm2' (l:concrete_st) (o1 o2:op_t) (l1' l2':log) (last1 last2:op_t)
+  : Lemma (requires fst o1 <> fst o2 /\ ~ (comm_ops o1 o2) /\ Fst_snd? (rc o2 o1) /\ comm_ops o1 last1 /\
+                    fst last1 <> fst last2 /\ comm_ops last1 last2 /\
+                    length l2' = 0 /\ length l1' > 0 /\
+                    (let pre1, lastl1 = un_snoc l1' in
+                     eq (merge (do l o1) (apply_log (do l o1) l1') (do (apply_log (do (do l o2) o1) l2') last2))
+                        (do (merge (do l o1) (apply_log (do l o1) l1') (apply_log (do (do l o2) o1) l2')) last2)))
+          (ensures eq (merge (do l o1) (do (apply_log (do l o1) l1') last1) (do (apply_log (do (do l o2) o1) l2') last2))
+                      (do (merge (do l o1) (do (apply_log (do l o1) l1') last1) (apply_log (do (do l o2) o1) l2')) last2)) = ()
+
+
+let rec prop3_base_rc (l:st) (o1 o2:op_t) (last1 last2:op_t)
+  : Lemma (requires fst o1 <> fst o2 /\ ~ (comm_ops o1 o2) /\ Fst_snd? (rc o2 o1) /\
+                    fst last1 <> fst last2 /\ ~ (comm_ops last1 last2) /\ Fst_snd? (rc last1 last2))
+          (ensures eq (merge (v_of l) (do (do (v_of l) o1) last1) (do (do (do (v_of l) o2) o1) last2))
+                      (do (merge (v_of l) (do (do (v_of l) o1) last1) (do (do (v_of l) o2) o1)) last2))
+          (decreases length (ops_of l)) =
+  if length (ops_of l) = 0 then ()
+  else prop3_base_rc (inverse_st l) o1 o2 last1 last2
+
+let prop4_base_comm (l:st) (o1 o2:op_t) (last1 last2:op_t)
+  : Lemma (requires fst o1 <> fst o2 /\ ~ (comm_ops o1 o2) /\ Fst_snd? (rc o2 o1) /\ comm_ops last1 o1 /\
+                    fst last1 <> fst last2 /\ comm_ops last1 last2 /\ not (reorder last2 (create 1 last1)))
+          (ensures eq (merge (v_of l) (do (do (v_of l) o1) last1) (do (do (do (v_of l) o2) o1) last2))
+                      (do (merge (v_of l) (do (do (v_of l) o1) last1) (do (do (v_of l) o2) o1)) last2)) = ()
+     
+let prop3_ind_rc1 (l:concrete_st) (o1 o2:op_t) (l1' l2':log) (last1 last2:op_t)
+  : Lemma (requires fst o1 <> fst o2 /\ ~ (comm_ops o1 o2) /\ Fst_snd? (rc o2 o1) /\
+                    fst last1 <> fst last2 /\ ~ (comm_ops last1 last2) /\ Fst_snd? (rc last1 last2) /\
+                    length l2' > 0 /\ 
+                    (let pre2, lastl2 = un_snoc l2' in
+                     eq (merge l (do (apply_log (do l o1) l1') last1) (do (apply_log (do (do l o2) o1) pre2) last2))
+                        (do (merge l (do (apply_log (do l o1) l1') last1) (apply_log (do (do l o2) o1) pre2)) last2)))
+          (ensures eq (merge l (do (apply_log (do l o1) l1') last1) (do (apply_log (do (do l o2) o1) l2') last2))
+                      (do (merge l (do (apply_log (do l o1) l1') last1) (apply_log (do (do l o2) o1) l2')) last2)) = admit()
+
+let prop3_ind_rc2 (l:concrete_st) (o1 o2:op_t) (l1' l2':log) (last1 last2:op_t)
+  : Lemma (requires fst o1 <> fst o2 /\ ~ (comm_ops o1 o2) /\ Fst_snd? (rc o2 o1) /\
+                    fst last1 <> fst last2 /\ ~ (comm_ops last1 last2) /\ Fst_snd? (rc last1 last2) /\
+                    length l2' = 0 /\ length l1' > 0 /\
+                    (let pre1, lastl1 = un_snoc l1' in
+                     eq (merge l (do (apply_log (do l o1) pre1) last1) (do (apply_log (do (do l o2) o1) l2') last2))
+                        (do (merge l (do (apply_log (do l o1) pre1) last1) (apply_log (do (do l o2) o1) l2')) last2)))
+          (ensures eq (merge l (do (apply_log (do l o1) l1') last1) (do (apply_log (do (do l o2) o1) l2') last2))
+                      (do (merge l (do (apply_log (do l o1) l1') last1) (apply_log (do (do l o2) o1) l2')) last2)) = ()
+
+let prop4_ind_comm1 (l:concrete_st) (o1 o2:op_t) (l1' l2':log) (last1 last2:op_t)
+  : Lemma (requires fst o1 <> fst o2 /\ ~ (comm_ops o1 o2) /\ Fst_snd? (rc o2 o1) /\ comm_ops o1 last1 /\
+                    fst last1 <> fst last2 /\ comm_ops last1 last2 /\
+                    length l2' > 0 /\ 
+                    (let pre2, lastl2 = un_snoc l2' in
+                     eq (merge l (do (apply_log (do l o1) l1') last1) (do (apply_log (do (do l o2) o1) pre2) last2))
+                        (do (merge l (do (apply_log (do l o1) l1') last1) (apply_log (do (do l o2) o1) pre2)) last2)))
+          (ensures eq (merge l (do (apply_log (do l o1) l1') last1) (do (apply_log (do (do l o2) o1) l2') last2))
+                      (do (merge l (do (apply_log (do l o1) l1') last1) (apply_log (do (do l o2) o1) l2')) last2)) = admit()
+
+let prop4_ind_comm2 (l:concrete_st) (o1 o2:op_t) (l1' l2':log) (last1 last2:op_t)
+  : Lemma (requires fst o1 <> fst o2 /\ ~ (comm_ops o1 o2) /\ Fst_snd? (rc o2 o1) /\ comm_ops o1 last1 /\
+                    fst last1 <> fst last2 /\ comm_ops last1 last2 /\
+                    length l2' = 0 /\ length l1' > 0 /\
+                    (let pre1, lastl1 = un_snoc l1' in
+                     eq (merge l (apply_log (do l o1) l1') (do (apply_log (do (do l o2) o1) l2') last2))
+                        (do (merge l (apply_log (do l o1) l1') (apply_log (do (do l o2) o1) l2')) last2)))
+          (ensures eq (merge l (do (apply_log (do l o1) l1') last1) (do (apply_log (do (do l o2) o1) l2') last2))
+                      (do (merge l (do (apply_log (do l o1) l1') last1) (apply_log (do (do l o2) o1) l2')) last2)) = ()*)
+                      
 ////////////////////////////////////////////////////////////////
